Variable name tweak for deriv_ty

nola/judg.v
@@ -15,7 +15,7 @@ Structure judg := Judg {
     (∀ i, judg_data i → Prop) → ∀ i, judg_data i → Prop;
 }.
 Add Printing Constructor judg.
-Arguments judg_sem {JU} φ i J : rename.
+Arguments judg_sem {JU} d i J : rename.
 
 (** Derivability predicate *)
 Notation deriv_ty JU := (∀ i, JU.(judg_data) i → Prop).
@@ -27,18 +27,18 @@ Notation pderiv_ty JU := (deriv_ty JU → deriv_ty JU).
 Definition Falseᵈ {JU} : deriv_ty JU := λ _ _, False.
 Notation "⊥ᵈ" := Falseᵈ : nola_scope.
 
-Definition orᵈ {JU} (φ ψ : deriv_ty JU) : deriv_ty JU := λ i J, φ i J ∨ ψ i J.
+Definition orᵈ {JU} (d d' : deriv_ty JU) : deriv_ty JU := λ i J, d i J ∨ d' i J.
 Infix "∨ᵈ" := orᵈ (at level 50, left associativity) : nola_scope.
 
-Definition apporᵈ {JU} (δ : pderiv_ty JU) (φ : deriv_ty JU) : deriv_ty JU :=
-  δ φ ∨ᵈ φ.
+Definition apporᵈ {JU} (δ : pderiv_ty JU) (d : deriv_ty JU) : deriv_ty JU :=
+  δ d ∨ᵈ d.
 Infix "$∨ᵈ" := apporᵈ (at level 50, left associativity) : nola_scope.
 
-Definition implᵈ {JU} (φ ψ : deriv_ty JU) : Prop := ∀ i J, φ i J → ψ i J.
+Definition implᵈ {JU} (d d' : deriv_ty JU) : Prop := ∀ i J, d i J → d' i J.
 Infix "→ᵈ" := implᵈ (at level 99, right associativity) : nola_scope.
 
-Definition implᵈ_low {JU} (i : JU.(judg_idx)) (φ ψ : deriv_ty JU) : Prop :=
-  ∀ j, j ≺ i → ∀ K, φ j K → ψ j K.
+Definition implᵈ_low {JU} (i : JU.(judg_idx)) (d d' : deriv_ty JU) : Prop :=
+  ∀ j, j ≺ i → ∀ K, d j K → d' j K.
 Infix "→ᵈ[≺ i ]" := (implᵈ_low i) (at level 99, right associativity)
   : nola_scope.
 
@@ -48,18 +48,18 @@ Infix "→ᵈ[≺ i ]" := (implᵈ_low i) (at level 99, right associativity)
 Record derivy_gen (JU : judg) (self : pderiv_ty JU → Prop) (δ : pderiv_ty JU)
   : Prop := {
   (** [δ] is monotone over the coinductive hypothesis *)
-  derivy_gen_mono {φ ψ : deriv_ty JU} : (φ →ᵈ ψ) → δ φ →ᵈ δ ψ;
+  derivy_gen_mono {d d' : deriv_ty JU} : (d →ᵈ d') → δ d →ᵈ δ d';
   (** [δ] can accumulate coinductive hypotheses *)
-  derivy_gen_acc {φ} (res : deriv_ty JU) : (res →ᵈ δ (φ ∨ᵈ res)) → res →ᵈ δ φ;
-  (** [δ φ i J] can be proved by semantics *)
-  derivy_gen_bysem {φ i J} :
-    (∀ δ', self δ' → (δ φ i →₁ judg_sem (δ' ⊥ᵈ) i) → (δ $∨ᵈ φ →ᵈ δ' ⊥ᵈ) →
+  derivy_gen_acc {d} (res : deriv_ty JU) : (res →ᵈ δ (d ∨ᵈ res)) → res →ᵈ δ d;
+  (** [δ d i J] can be proved by semantics *)
+  derivy_gen_bysem {d i J} :
+    (∀ δ', self δ' → (δ d i →₁ judg_sem (δ' ⊥ᵈ) i) → (δ $∨ᵈ d →ᵈ δ' ⊥ᵈ) →
       (δ' ⊥ᵈ →ᵈ[≺ i] judg_sem (δ' ⊥ᵈ)) → judg_sem (δ' ⊥ᵈ) i J) →
-    δ φ i J
+    δ d i J
 }.
 #[export] Instance derivy_gen_mono₁₁ {JU} : Mono₁₁ (derivy_gen JU).
 Proof.
-  move=> D E DE δ [?? bysem]. split; [done|done|]=> φ i J H.
+  move=> D E DE δ [?? bysem]. split; [done|done|]=> d i J H.
   apply bysem=> δ' /DE. apply H.
 Qed.
 
@@ -67,43 +67,43 @@ Qed.
 Definition derivy (JU : judg) : pderiv_ty JU → Prop := mu (derivy_gen JU).
 Existing Class derivy.
 
-(** [inderivy JU δ' δ φ i] : Characterization of a derivability predicate
-  in [δ φ i]'s [derivy_bysem] *)
-Class inderivy (JU : judg) (δ' δ : pderiv_ty JU) (φ : deriv_ty JU)
+(** [inderivy JU δ' δ d i] : Characterization of a derivability predicate
+  in [δ d i]'s [derivy_bysem] *)
+Class inderivy (JU : judg) (δ' δ : pderiv_ty JU) (d : deriv_ty JU)
   (i : JU.(judg_idx)) : Prop := {
   (** [δ'] satisfies [derivy] *)
   inderivy_derivy :: derivy JU δ';
-  (** Interpret [δ φ i] as [judg_sem (δ' ⊥ᵈ) i] *)
-  inderivy_sem : δ φ i →₁ judg_sem (δ' ⊥ᵈ) i;
-  (** Turn [δ $∨ᵈ φ] into [δ' ⊥ᵈ] *)
-  inderivy_turn : δ $∨ᵈ φ →ᵈ δ' ⊥ᵈ;
+  (** Interpret [δ d i] as [judg_sem (δ' ⊥ᵈ) i] *)
+  inderivy_sem : δ d i →₁ judg_sem (δ' ⊥ᵈ) i;
+  (** Turn [δ $∨ᵈ d] into [δ' ⊥ᵈ] *)
+  inderivy_turn : δ $∨ᵈ d →ᵈ δ' ⊥ᵈ;
   (** Interpret [δ' ⊥ᵈ j] as [judg_sem (δ' ⊥ᵈ) j] for [j ≺ i] *)
   inderivy_semlow : δ' ⊥ᵈ →ᵈ[≺ i] judg_sem (δ' ⊥ᵈ);
 }.
 
 (** Lemmas for [derivy] *)
-Lemma derivy_mono `{D : derivy JU δ} {φ ψ} : (φ →ᵈ ψ) → δ φ →ᵈ δ ψ.
+Lemma derivy_mono `{D : derivy JU δ} {d d'} : (d →ᵈ d') → δ d →ᵈ δ d'.
 Proof. move: D=> /mu_unfold [mono _ _]. apply mono. Qed.
-Lemma derivy_acc `{D : derivy JU δ} {φ} res :
-  (res →ᵈ δ (φ ∨ᵈ res)) → res →ᵈ δ φ.
+Lemma derivy_acc `{D : derivy JU δ} {d} res :
+  (res →ᵈ δ (d ∨ᵈ res)) → res →ᵈ δ d.
 Proof. move: D=> /mu_unfold [_ acc _]. apply acc. Qed.
-Lemma derivy_bysem `{D : derivy JU δ} {φ i J} :
-  (∀ δ', inderivy JU δ' δ φ i → judg_sem (δ' ⊥ᵈ) i J) → δ φ i J.
+Lemma derivy_bysem `{D : derivy JU δ} {d i J} :
+  (∀ δ', inderivy JU δ' δ d i → judg_sem (δ' ⊥ᵈ) i J) → δ d i J.
 Proof. move: D=> /mu_unfold [_ _ bysem]=> H. apply bysem=> *. by apply H. Qed.
 
 (** Lemmas for [inderivy] *)
-Lemma inderivy_turn_l `{inderivy JU δ' δ φ i} : δ φ →ᵈ δ' ⊥ᵈ.
+Lemma inderivy_turn_l `{inderivy JU δ' δ d i} : δ d →ᵈ δ' ⊥ᵈ.
 Proof. move=> *. apply inderivy_turn. by left. Qed.
-Lemma inderivy_turn_r `{inderivy JU δ' δ φ i} : φ →ᵈ δ' ⊥ᵈ.
+Lemma inderivy_turn_r `{inderivy JU δ' δ d i} : d →ᵈ δ' ⊥ᵈ.
 Proof. move=> *. apply inderivy_turn. by right. Qed.
-Lemma inderivy_turn_semlow `{inderivy JU δ' δ φ i} :
-  δ $∨ᵈ φ →ᵈ[≺ i] judg_sem (δ' ⊥ᵈ).
+Lemma inderivy_turn_semlow `{inderivy JU δ' δ d i} :
+  δ $∨ᵈ d →ᵈ[≺ i] judg_sem (δ' ⊥ᵈ).
 Proof. move=> *. apply inderivy_semlow; by [|apply inderivy_turn]. Qed.
-Lemma inderivy_turn_semlow_l `{inderivy JU δ' δ φ i} :
-  δ φ →ᵈ[≺ i] judg_sem (δ' ⊥ᵈ).
+Lemma inderivy_turn_semlow_l `{inderivy JU δ' δ d i} :
+  δ d →ᵈ[≺ i] judg_sem (δ' ⊥ᵈ).
 Proof. move=> *. apply inderivy_turn_semlow; by [|left]. Qed.
-Lemma inderivy_turn_semlow_r `{inderivy JU δ' δ φ i} :
-  φ →ᵈ[≺ i] judg_sem (δ' ⊥ᵈ).
+Lemma inderivy_turn_semlow_r `{inderivy JU δ' δ d i} :
+  d →ᵈ[≺ i] judg_sem (δ' ⊥ᵈ).
 Proof. move=> *. apply inderivy_turn_semlow; by [|right]. Qed.
 
 (** ** [deriv]: Derivability *)
@@ -125,33 +125,33 @@ Record deriv_aty (JU : judg) := DerivAty {
 Arguments DerivAty {_} _ _.
 
 (** Conversion between [deriv_aty JU → Prop] and [deriv_ty JU] *)
-Definition deriv_curry {JU} (φ : deriv_aty JU → Prop) : deriv_ty JU :=
-  λ i J, φ (DerivAty i J).
-Definition deriv_uncurry {JU} (φ : deriv_ty JU) : deriv_aty JU → Prop :=
-  λ '(DerivAty i J), φ i J.
+Definition deriv_curry {JU} (d : deriv_aty JU → Prop) : deriv_ty JU :=
+  λ i J, d (DerivAty i J).
+Definition deriv_uncurry {JU} (d : deriv_ty JU) : deriv_aty JU → Prop :=
+  λ '(DerivAty i J), d i J.
 
 (** Modified [deriv_gen] *)
-Definition deriv_gen' JU (φ : deriv_aty JU → Prop) : deriv_aty JU → Prop :=
-  deriv_uncurry (deriv_gen JU (deriv_curry φ)).
+Definition deriv_gen' JU (d : deriv_aty JU → Prop) : deriv_aty JU → Prop :=
+  deriv_uncurry (deriv_gen JU (deriv_curry d)).
 #[export] Instance deriv_gen'_mono JU : Mono₁₁ (deriv_gen' JU).
 Proof.
-  move=> φ ψ φψ [i J] +. move: i J. fix FIX 3=> i J [[der[derto big]]].
+  move=> d d' dd' [i J] +. move: i J. fix FIX 3=> i J [[der[derto big]]].
   split. exists der. split. { move=> K /derto. apply FIX. }
-  move=> δ' ?? turn ?. apply big; [done|done| |done]=> j K /φψ. apply turn.
+  move=> δ' ?? turn ?. apply big; [done|done| |done]=> j K /dd'. apply turn.
 Qed.
 
 (** [deriv]: Derivability *)
-Definition deriv (JU : judg) (φ : deriv_ty JU) : deriv_ty JU :=
-  deriv_curry (pnu (deriv_gen' JU) (deriv_uncurry φ)).
+Definition deriv (JU : judg) (d : deriv_ty JU) : deriv_ty JU :=
+  deriv_curry (pnu (deriv_gen' JU) (deriv_uncurry d)).
 
 (** [deriv] satisfies [derivy] *)
 #[export] Instance deriv_derivy {JU} : derivy JU (deriv JU).
 Proof.
   apply mu_fold. split.
-  - move=> φ ψ φψ i J. apply pnu_mono=> [[j K]] /φψ. done.
-  - move=> φ res resto i J ?. apply (pnu_acc (deriv_uncurry res)); [|done].
+  - move=> d d' dd' i J. apply pnu_mono=> [[j K]] /dd'. done.
+  - move=> d res resto i J ?. apply (pnu_acc (deriv_uncurry res)); [|done].
     move=> [j K] /resto. done.
-  - move=> φ i J H. apply pnu_fold. split. exists (deriv JU φ i).
+  - move=> d i J H. apply pnu_fold. split. exists (deriv JU d i).
     split. { by move=> J' /pnu_unfold. } { move=> δ'. apply H. }
 Qed.
 
